fstar/code/arch/x64/X64.Vale.QuickCode.fst
@@ -67,27 +67,13 @@ let va_mod_reg_opr64 (o:operand) : mod_t =
 
 let quickProc_wp (a:Type0) : Type u#1 = (s0:state) -> (wp_continue:state -> a -> Type0) -> Type0
 
-let k_true (#a:Type0) (_:state) (_:a) = True
+let t_ensure (#a:Type0) (c:va_code) (mods:mods_t) (wp:quickProc_wp a) (s0:state) (k:(state -> a -> Type0)) =
+  fun (sM, f0, g) -> eval_code c s0 f0 sM /\ update_state_mods mods sM s0 == sM /\ k sM g
 
-let t_monotone (#a:Type0) (c:va_code) (wp:quickProc_wp a) : Type =
-  s0:state -> k1:(state -> a -> Type0) -> k2:(state -> a -> Type0) -> Lemma
-    (requires (forall (s:state) (g:a). k1 s g ==> k2 s g))
-    (ensures wp s0 k1 ==> wp s0 k2)
-
-let t_compute (#a:Type0) (c:va_code) (wp:quickProc_wp a) : Type =
-  s0:state -> Ghost (state * va_fuel * a)
-    (requires wp s0 k_true)
-    (ensures fun _ -> True)
-
-let t_ensure (#a:Type0) (c:va_code) (mods:mods_t) (wp:quickProc_wp a) (monotone:t_monotone c wp) (compute:t_compute c wp) (s0:state) (k:(state -> a -> Type0){wp s0 k}) =
-  monotone s0 k k_true;
-  let (sM, f0, g) = compute s0 in
-  eval_code c s0 f0 sM /\ update_state_mods mods sM s0 == sM /\ k sM g
-
-let t_proof (#a:Type0) (c:va_code) (mods:mods_t) (wp:quickProc_wp a) (monotone:t_monotone c wp) (compute:t_compute c wp) : Type =
-  s0:state -> k:(state -> a -> Type0) -> Lemma
+let t_proof (#a:Type0) (c:va_code) (mods:mods_t) (wp:quickProc_wp a) : Type =
+  s0:state -> k:(state -> a -> Type0) -> Ghost (state * va_fuel * a)
     (requires wp s0 k)
-    (ensures t_ensure c mods wp monotone compute s0 k)
+    (ensures t_ensure c mods wp s0 k)
 
 // Code that returns a ghost value of type a
 [@va_qattr]
@@ -96,9 +82,7 @@ noeq type quickCode (a:Type0) : va_code -> Type =
     c:va_code ->
     mods:mods_t ->
     wp:quickProc_wp a ->
-    monotone:t_monotone c wp ->
-    compute:t_compute c wp ->
-    proof:t_proof c mods wp monotone compute ->
+    proof:t_proof c mods wp ->
     quickCode a c
 
 unfold let va_quickCode = quickCode
